Finish decidability of halting for small fractran

theories/FRACTRAN/Utils/reversibility_facts.v
@@ -1,25 +1,16 @@
-Require Import List Arith Lia.
+Require Import List Arith Lia Permutation.
 Import ListNotations.
 
 From Undecidability.Shared.Libs.DLW
-     Require Import gcd prime.
+     Require Import gcd prime Utils.utils_tac.
 
 From Undecidability.FRACTRAN
-     Require Import FRACTRAN.
+     Require Import FRACTRAN fractran_utils.
 
 From Undecidability.Synthetic
      Require Import Definitions.
 
 Section ListFacts.
-
-  (* Definition any := existsb id. *)
-
-  (* Definition zipWith {X Y Z} (f : X*Y -> Z) xs ys := map f (combine xs ys). *)
-
-  (* Lemma any_zipWith_p {X Y} (p : X*Y -> bool) (xs : list X) (ys : list Y) : *)
-  (*   any (zipWith p xs ys) = true <-> *)
-  (*     exists (i : nat) x y, nth_error xs i = Some x /\ nth_error ys i = Some y /\ p (x,y) = true. *)
-  (* Admitted. *)
 
   Lemma length_one_iff_singleton {X} (l : list X) : length l = 1 <-> exists x, l = [x].
   Proof.
@@ -30,112 +21,246 @@ Section ListFacts.
     - intros [y]. now inversion H.
   Qed.
 
+  Lemma length_at_least_0 {X} (l : list X) : length l >= 0.
+  Proof.
+    induction l as [|a l IHl]; simpl; lia.
+  Qed.
+
 End ListFacts.
 
-Section redundant_FRAC.
+(* Some facts about prime factors due to Andrej *)
+Section Prime_factors.
 
-  Definition red_FRAC (l : list (nat * nat)) :=
-    exists c1 d1 c2 d2 l1 l2 l3, l1 ++ [(c1, d1)] ++ l2 ++ [(c2, d2)] ++ l3 = l /\ divides d1 d2.
-
-  Definition nred_FRAC (l : list (nat * nat)) :=
-    forall c1 d1 c2 d2 l1 l2 l3, l1 ++ [(c1, d1)] ++ l2 ++ [(c2, d2)] ++ l3 = l -> ~ divides d1 d2.
-
-  Lemma nred_not_red l : nred_FRAC l -> ~ red_FRAC l.
+  Lemma count_occ_app H (n : nat) l1 l2:
+    count_occ H (l1 ++ l2) n =
+    count_occ H l1 n + count_occ H l2 n.
   Proof.
-    unfold nred_FRAC.
-    intros H [c1 [d1 [c2 [d2 [l1 [l2 [l3 [H1 H2]]]]]]]].
-    eapply H.
-    - exact H1.
-    - exact H2.
+    revert l2. induction l1; [easy|].
+    intro l2. cbn. rewrite IHl1.
+    now destruct (H a n).
   Qed.
 
-  Lemma l0_nred l : length l = 0 -> nred_FRAC l.
+  Notation lprod := (fold_right mult 1).
+  Infix "<d" := divides (at level 70, no associativity).
+
+  Fact lprod_insert a ld l1c l2c :
+    lprod (ld) <d lprod (l1c ++ l2c) -> lprod (a :: ld) <d lprod (l1c ++ a :: l2c).
   Proof.
-    intros H%length_zero_iff_nil. rewrite H.
-    intros c1 d1 c2 d2 l1 l2 l3 H1 Hdiv.
-    do 3 rewrite app_assoc in H1.
-    apply app_eq_nil in H1 as [H1 _].
-    apply app_eq_nil in H1 as [_ H3].
-    congruence.
+    rewrite !lprod_app. cbn. unfold divides.
+    intros [p Hp]. exists p. nia.
   Qed.
 
-  Lemma l1_nred l : length l = 1 -> nred_FRAC l.
+  Lemma prime_key_div {lc ld} :
+    ~ (divides (lprod ld) (lprod lc)) ->
+    Forall prime lc -> Forall prime ld ->
+    exists (p : nat), prime p /\ count_occ Nat.eq_dec lc p < count_occ Nat.eq_dec ld p.
   Proof.
-    intros H%length_one_iff_singleton. destruct H as [x H]. rewrite H.
-    intros c1 d1 c2 d2 l1 l2 l3 H1 Hdiv.
-    do 3 rewrite app_assoc in H1.
-    apply app_eq_unit in H1 as [[H1 _]|[H1 _]].
-    - apply app_eq_nil in H1 as [_ H1]. congruence.
-    - apply app_eq_unit in H1 as [[H1 _]|[_ H3]].
-      + apply app_eq_nil in H1 as [H1 _].
-        apply app_eq_nil in H1 as [_ H1]. congruence.
-      + congruence.
+    revert lc. induction ld as [|a ld IHld].
+    - intros lc H. exfalso. apply H.
+      exists (lprod lc). cbn. lia.
+    - intros lc H Hlc Hld'.
+      pose proof (Ha := Forall_inv Hld').
+      pose proof (Hld := Forall_inv_tail Hld').
+      destruct (in_dec Nat.eq_dec a lc) as [Halc|Halc].
+      + apply in_split in Halc as [l1c [l2c ?]]. subst lc.
+        assert (H' : not (lprod (ld) <d lprod (l1c ++ l2c)))
+          by now intros ?%(lprod_insert a).
+        assert (H'lc : Forall prime (l1c ++ l2c)).
+        { revert Hlc. rewrite !Forall_app.
+          now intros [? ? %Forall_inv_tail]. }
+        specialize (IHld _ H' H'lc Hld).
+        destruct IHld as [p [? Hp]].
+        exists p. split; [assumption|].
+        revert Hp. rewrite !count_occ_app. cbn.
+        destruct (Nat.eq_dec); lia.
+      + exists a. split; [assumption|].
+        apply (count_occ_not_In Nat.eq_dec) in Halc.
+        rewrite count_occ_cons_eq, Halc; lia.
   Qed.
 
-End redundant_FRAC.
+  Definition count_pow (p n : nat) : nat :=
+    let (l, _) := (@prime_decomp (S n) (Nat.neq_succ_0 n))
+     in count_occ Nat.eq_dec l p.
 
-Definition reg_frac '(c,d) := c <> 0 /\ d <> 0.
+  Infix "~p" := (@Permutation _) (at level 70).
 
-Section Small_FRAC_halt_dec.
-
-  Variable (l : list (nat * nat)) (Hreg : Forall reg_frac l).
-
-  Lemma fractran_halt_dec_l0 : length l = 0 -> decidable (fractran_terminates l).
+  Lemma Permutation_count_occ x l1 l2 : l1 ~p l2 ->
+    count_occ Nat.eq_dec l1 x = count_occ Nat.eq_dec l2 x.
   Proof.
-    intros H%length_zero_iff_nil.
-    exists (fun _ => true). intros x. split.
-    - now intros Hf.
-    - intros _.
-      exists x. split.
-      + now exists 0.
-      + intros z H2. now destruct H2.
+    revert l2. induction l1.
+    - intros l2. cbn. intros ? %Permutation_nil. now subst.
+    - intros l2. intros H %Permutation_sym.
+      pose proof (H' := H).
+      apply Permutation_vs_cons_inv in H' as [l2' [l2'' ?]]. subst.
+      apply Permutation_sym, Permutation_cons_app_inv, IHl1 in H.
+      rewrite count_occ_app in H.
+      cbn. destruct Nat.eq_dec.
+      + rewrite count_occ_app. cbn.
+        destruct Nat.eq_dec; lia.
+      + rewrite count_occ_app. cbn.
+        destruct Nat.eq_dec; lia.
   Qed.
 
-  Lemma fractran_halt_dec_l1 : length l = 1 -> decidable (fractran_terminates l).
+  Lemma prime_key_div' c d (Hc : c <> 0) (Hd : d <> 0) :
+    ~ (divides d c) ->
+    exists p,
+      (forall x y (Hx : x <> 0) (Hy : y <> 0),
+        x * c = y * d -> count_pow p (pred y) < count_pow p (pred x)).
   Proof.
-    intros H%length_one_iff_singleton. destruct H as [(c,d) H]. rewrite H.
-    exists (fun x => match x with 0 => false | _ => if divides_dec c d then false else true end).
-    intros x. split.
-    - intros [y [[n Hy] Hs]].
-      destruct (divides_dec c d) as [[k Hk] | Hndiv].
-      + exfalso. apply Hs with (z:=k*y). constructor. lia.
-      + destruct x.
-        * exfalso. apply Hs with (z:=0). enough (y = 0) by (subst; constructor; lia).
-          induction n as [|n IHn].
-          -- now simpl in Hy.
-          -- apply IHn. simpl in Hy. destruct Hy as [y0 [Hy1 Hy2]].
-             enough (y0 = 0) by (subst; apply Hy2).
-             inversion Hy1; subst. enough (d <> 0) by lia.
-             ++ inversion Hreg. subst. apply H1.
-             ++ inversion H6.
-        * reflexivity.
-    - destruct (divides_dec c d) as [[k Hk]|Hndiv].
-      + destruct x; now intros.
-      + destruct x.
-        * now intros.
-        * intros _. (pose proof (@prime_decomp c)).
+    pose proof (@prime_decomp c Hc) as [lc [Hclc Hlc]].
+    pose proof (@prime_decomp d Hd) as [ld [Hdld Hld]].
+    subst. intros H. apply prime_key_div in H as [p [? Hp]]; [|assumption ..].
+    exists p. intros x y Hx Hy. unfold count_pow.
+    destruct (@prime_decomp (S (pred x)) _) as [lx [Hxlx Hlx]].
+    destruct (@prime_decomp (S (pred y)) _) as [ly [Hyly Hly]].
+    assert (S (pred x) = x) as H'x by lia.
+    assert (S (pred y) = y) as H'y by lia.
+    rewrite H'x in Hxlx. rewrite H'y in Hyly.
+    subst. rewrite <- !lprod_app.
+    intros E. apply prime_decomp_uniq in E; [|now rewrite Forall_app ..].
+    apply (Permutation_count_occ p) in E. rewrite !count_occ_app in E. lia.
+  Qed.
+
+End Prime_factors.
+
+Section Fractran_Facts.
+
+  Lemma fractran_step_zero y l (Hl : l <> nil) (Hlreg : fractran_regular l) :
+    l /F/ 0 → y <-> y = 0.
+  Proof.
+    split.
+    - induction l as [|(c,d) l IHl]; [congruence|]. inversion 1; subst.
+      + apply Forall_inv in Hlreg. simpl in Hlreg. lia.
+      + apply IHl; auto.
+        * intros H2; subst. inversion H6.
+        * now apply Forall_inv_tail with (a:=(c,d)).
+    - intros ->. destruct l as [|(p,q) l]; [congruence|].
+      constructor. lia.
+  Qed.
+
+  Lemma fractran_steps_zero x l (Hl : l <> nil) (Hlreg : fractran_regular l) :
+    forall n, fractran_steps l n 0 x <-> x = 0.
+  Proof.
+    induction n as [|n IHn]; simpl; [split; auto|]. split.
+    - intros [y [Hy Hs]]. apply IHn. apply fractran_step_zero in Hy; subst; auto.
+    - intros ->. exists 0. split; [|now apply IHn].
+      apply fractran_step_zero; auto.
+  Qed.
+
+  Corollary fractran_nstop_zero l (Hl : l <> nil) (Hlreg : fractran_regular l) :
+    ~ l /F/ 0 ↓.
+  Proof.
+    intros [y [[n Hy] Hstop]]. apply fractran_steps_zero in Hy; subst; auto.
+    destruct l as [| (c,d) l]; subst; [congruence|].
+    apply (Hstop 0). constructor. lia.
+  Qed.
+
+  Corollary fractran_singleton_steps_zero x c d (Hd : d <> 0) :
+    forall n, fractran_steps [(c,d)] n 0 x <-> x = 0.
+  Proof.
+    apply fractran_steps_zero; [congruence|].
+    constructor; auto.
+  Qed.
+
+  Corollary fractran_singleton_nstop_zero c d (Hd : d <> 0) : ~ [(c,d)] /F/ 0 ↓.
+  Proof.
+    apply fractran_nstop_zero; [congruence|].
+    apply Forall_cons; auto.
+  Qed.
+
+  Lemma fractran_step_nzero x y c d (Hx : x <> 0) (Hc : c <> 0) (Hd : d <> 0) :
+    [(c,d)] /F/ x → y -> y <> 0.
+  Proof.
+    inversion 1; subst.
+    - lia.
+    - inversion H6.
+  Qed.
+
+  Lemma fractran_singleton_ndiv_stop_S x c d (Hx : x <> 0) (Hc : c <> 0) (Hd : d <> 0) :
+    ~ divides d c -> [(c,d)] /F/ x ↓.
+  Proof.
+    intros Hndiv%prime_key_div'; [|exact Hc|exact Hd].
+    destruct Hndiv as [p H]. revert Hx.
+    induction on x as IH with measure (count_pow p (pred x)).
+    intros Hx. destruct (fractran_step_dec [(c,d)] x) as [[y Hxy]|Hs].
+    - assert (Hy : y <> 0) by (apply (fractran_step_nzero x _ c d); auto).
+      inversion Hxy; subst.
+      + specialize (H x y Hx Hy ltac: (lia)). specialize (IH y).
+        apply IH in H as [y' [[n Hyy'] Hs']]; [|exact Hy]. exists y'. split; [|exact Hs'].
+        exists (1+n). simpl. exists y. auto.
+      + inversion H6.
+    - exists x. split; [|exact Hs].
+      exists 0. now simpl.
+  Qed.
+
+  Lemma redundant_fractran_step l1 l2 l3 c1 d1 c2 d2 x y : divides d1 d2 ->
+    l1 ++ [(c1,d1)] ++ l2 ++ [(c2,d2)] ++ l3 /F/ x → y <-> l1 ++ [(c1,d1)] ++ l2 ++ l3 /F/ x → y.
+  Proof.
   Admitted.
 
-  (* Lemma foo : *)
-  (*   exists (p k : nat), prime p -> divides (p^k) d -> ~ divides (p^k) c -> *)
-  (*                       forall x y lx ly, l /F/ x → y -> x = fold_right mult 1 lx -> Forall prime lx -> *)
-  (*                       y = fold_right mult 1 ly -> Forall prime ly -> count_occ ly p < count_occ lx p *)
+  (* forall l, if l is not redundant -> length l >= 2 -> not_reversible l *)
+  (* forall l, length l >= 2 -> reversible l -> redundant_fractran l *)
 
-  Lemma fractran_halt_dec_le2 : (length l = 0 \/ length l = 1) -> decidable (fractran_terminates l).
+End Fractran_Facts.
+
+Section Small_fractran_halt_dec.
+
+  Variable (c d : nat) (Hd : d <> 0).
+
+  Lemma fractran_empty_halt_dec : decidable (fun x => [] /F/ x ↓).
   Proof.
-    intros [H|H]; revert H.
-    - apply fractran_halt_dec_l0.
-    - apply fractran_halt_dec_l1.
+    exists (fun _ => true). intros x. split; [easy|].
+    intros _. exists x. split; [now exists 0|].
+    intros z H. inversion H.
   Qed.
 
-End Small_FRAC_halt_dec.
-
-Section Large_FRAC_not_reversible.
-
-  Variable (l : list (nat * nat)) (Hlen : length l > 1)
-           (Hred : nred_FRAC l) (Hreg : Forall reg_frac l).
-
-  Fact FRAC_not_rev : exists s t u, l /F/ s → u -> l /F/ t → u -> s <> t.
+  Lemma fractran_singleton_halt_dec : decidable (fun x => [(c,d)] /F/ x ↓).
   Proof.
+    exists (fun x => match x, c with
+                       0, _ => false
+                     | _, 0 => false
+                     | _, _ => if divides_dec c d then false else true
+                     end).
+    intros x. split.
+    - intros [y [[n Hy] Hstop]]. destruct x as [| x].
+      + apply fractran_steps_zero in Hy; subst; [|congruence|].
+        * specialize (Hstop 0). exfalso. apply Hstop. constructor. lia.
+        * apply Forall_cons; auto.
+      + destruct c as [| c'] eqn:Hc.
+        * specialize (Hstop 0). exfalso. apply Hstop. constructor. lia.
+        * destruct (divides_dec c d) as [[k Hk] | Hndiv] eqn:H; subst; [|now rewrite H].
+          exfalso. apply (Hstop (k*y)). constructor. lia.
+    - destruct x as [| x]; [congruence|].
+      destruct c as [| c'] eqn:Hc; [congruence|].
+      destruct (divides_dec c d) as [[k Hk] | Hndiv] eqn:H; subst.
+      + now rewrite H.
+      + intros _. apply fractran_singleton_ndiv_stop_S; auto.
+  Qed.
 
-End Large_FRAC_not_reversible.
+End Small_fractran_halt_dec.
+
+Theorem fractran_halt_dec_le2 l (Hl : fractran_regular l) :
+  (length l = 0 \/ length l = 1) -> decidable (fun x => l /F/ x ↓).
+Proof.
+  intros [ H%length_zero_iff_nil | H%length_one_iff_singleton ]; subst.
+  - exact fractran_empty_halt_dec.
+  - destruct H as [(c,d) H]. subst. apply Forall_inv in Hl. simpl in Hl.
+    now apply fractran_singleton_halt_dec.
+Qed.
+
+Section Redundant_fractran.
+
+  Definition fractran_redundant (l : list (nat * nat)) := exists l1 l2 l3 c1 d1 c2 d2,
+    l = l1 ++ [(c1,d1)] ++ l2 ++ [(c2,d2)] ++ l3 /\ divides d1 d2.
+
+End Redundant_fractran.
+
+Section Large_fractran_not_reversible.
+
+  Variable (l : list (nat * nat)) (Hreg : fractran_regular l) (Hlen : length l > 1).
+
+  Lemma large_fractran_not_reversible :
+    (forall s t u, l /F/ s → u -> l /F/ t → u -> s = t) -> fractran_redundant l.
+  Admitted.
+
+End Large_fractran_not_reversible.
